ProdEta is now configurable

formalization/config.v
@@ -10,5 +10,9 @@ Class SimpleProducts := {
   simpleproductsFlag : Type
 }.
 
+Class ProdEta := {
+  prodetaFlag : Type
+}.
+
 Inductive Yes : Type := yes.
 Inductive No : Type := .
