formalization/ett2ptt.v
@@ -9,6 +9,7 @@ Section Ett2Ptt.
 
 Context `{configReflection : config.Reflection}.
 Context `{configSimpleProducts : config.SimpleProducts}.
+Context `{ConfigProdEta : config.ProdEta}.
 
 (* Renaming ptt_sanity lemmata for readability. *)
 Definition ptt_sane_issubst := ptt_sanity.sane_issubst.
@@ -97,7 +98,7 @@ Proof.
 
      (* SubstComp *)
      - {
-         capply (@SubstComp _ _ _ G D E).
+         config apply @SubstComp with (D := D).
          - now apply sane_issubst.
          - now apply sane_issubst.
          - apply (ptt_sane_issubst sbs G D).
@@ -110,7 +111,7 @@ Proof.
 
      (* SubstCtxConv *)
      - {
-         capply (@SubstCtxConv _ _ _ G1 G2 D1 D2).
+         config apply @SubstCtxConv with (G1 := G1) (D1 := D1).
          - now apply sane_issubst.
          - now apply sane_eqctx.
          - now apply sane_eqctx.
@@ -129,7 +130,7 @@ Proof.
   { destruct P.
 
     (* TyCtxConv *)
-    { capply (@TyCtxConv _ _ _ G D).
+    { config apply @TyCtxConv with (G := G).
       - now apply sane_istype.
       - now apply sane_eqctx.
       - now apply (ptt_sane_eqctx G D), sane_eqctx.
@@ -137,7 +138,7 @@ Proof.
     }
 
     (* TySubst *)
-    { capply (@TySubst _ _ _ G D).
+    { config apply @TySubst with (D := D).
       - now apply sane_issubst.
       - now apply sane_istype.
       - now apply (ptt_sane_issubst sbs G D), sane_issubst.
@@ -188,7 +189,7 @@ Proof.
   { destruct P.
 
     (* TermTyConv *)
-    - { capply (@TermTyConv _ _ _ G A B).
+    - { config apply @TermTyConv with (A := A).
         - now apply sane_isterm.
         - now apply sane_eqtype.
         - now apply (@ptt_sane_isterm G u A), sane_isterm.
@@ -197,7 +198,7 @@ Proof.
       }
 
     (* TermCtxConv *)
-    - { capply (@TermCtxConv _ _ _ G D).
+    - { config apply @TermCtxConv with (G := G).
         - now apply sane_isterm.
         - now apply sane_eqctx.
         - now apply (@ptt_sane_isterm G u A), sane_isterm.
@@ -206,7 +207,7 @@ Proof.
       }
 
     (* TermSubst *)
-    - { capply (@TermSubst _ _ _ G D A).
+    - { config apply @TermSubst with (D := D).
         - now apply sane_issubst.
         - now apply sane_isterm.
         - now apply (@ptt_sane_issubst sbs G D), sane_issubst.
@@ -348,7 +349,7 @@ Proof.
       }
 
     (* CtxTrans *)
-    - { capply (@CtxTrans _ _ _ G D E).
+    - { config apply @CtxTrans with (D := D).
         - now apply (@ptt_sane_eqctx G D), sane_eqctx.
         - now apply (@ptt_sane_eqctx G D), sane_eqctx.
         - now apply (@ptt_sane_eqctx D E), sane_eqctx.
@@ -391,7 +392,7 @@ Proof.
       }
 
     (* SubstTrans *)
-    - { capply (@SubstTrans _ _ _ G D sb1 sb2 sb3).
+    - { config apply @SubstTrans with (sb2 := sb2).
         - now apply sane_eqsubst.
         - now apply sane_eqsubst.
         - now apply (@ptt_sane_eqsubst sb1 sb2 G D), sane_eqsubst.
@@ -402,7 +403,7 @@ Proof.
       }
 
     (* CongSubstZero *)
-    - { capply (@CongSubstZero _ _ _ G).
+    - { config apply @CongSubstZero with (G := G).
         - now apply sane_eqtype.
         - now apply sane_eqterm.
         - now apply (@ptt_sane_eqtype G A1 A2), sane_eqtype.
@@ -433,7 +434,7 @@ Proof.
       }
 
     (* CongSubstComp *)
-    - { capply (@CongSubstComp _ _ _ G D E).
+    - { config apply @CongSubstComp with (D := D).
         - now apply sane_eqsubst.
         - now apply sane_eqsubst.
         - now apply (@ptt_sane_eqsubst sbs1 sbs2 G D), sane_eqsubst.
@@ -446,7 +447,7 @@ Proof.
       }
 
     (* EqSubstCtxConv *)
-    - { capply (@EqSubstCtxConv _ _ _ G1 G2 D1 D2).
+    - { config apply @EqSubstCtxConv with (G1 := G1) (D1 := D1).
         - now apply sane_eqsubst.
         - now apply sane_eqctx.
         - now apply sane_eqctx.
@@ -459,7 +460,7 @@ Proof.
       }
 
     (* CompAssoc *)
-    - { capply (@CompAssoc _ _ _ G D E F).
+    - { config apply @CompAssoc with (D := D) (E := E).
         - now apply sane_issubst.
         - now apply sane_issubst.
         - now apply sane_issubst.
@@ -494,7 +495,7 @@ Proof.
       }
 
     (* CompShift *)
-    - { capply (@CompShift _ _ _ G D).
+    - { config apply @CompShift with (D := D).
         - now apply (@ptt_sane_issubst sbs G D), sane_issubst.
         - now apply (@ptt_sane_issubst sbs G D), sane_issubst.
         - now apply (@ptt_sane_istype E A), sane_istype.
@@ -523,7 +524,7 @@ Proof.
   { destruct P.
 
     (* EqTyCtxConv *)
-    { capply (@EqTyCtxConv _ _ _ G D).
+    { config apply @EqTyCtxConv with (G := G).
       - now apply sane_eqtype.
       - now apply sane_eqctx.
       - now apply (ptt_sane_eqtype G A B), sane_eqtype.
@@ -547,7 +548,7 @@ Proof.
     }
 
     (* EqTyTrans *)
-    { capply (@EqTyTrans _ _ _ G A B C).
+    { config apply @EqTyTrans with (B := B).
       - now apply sane_eqtype.
       - now apply sane_eqtype.
       - now apply (ptt_sane_eqtype G A B), sane_eqtype.
@@ -563,7 +564,7 @@ Proof.
     }
 
     (* EqTySubstComp *)
-    { capply (@EqTySubstComp _ _ _ G D E).
+    { config apply @EqTySubstComp with (D := D) (E := E).
       - now apply sane_istype.
       - now apply sane_issubst.
       - now apply sane_issubst.
@@ -573,7 +574,7 @@ Proof.
     }
 
     (* EqTySubstProd *)
-    { capply (@EqTySubstProd _ _ _ G D).
+    { config apply @EqTySubstProd with (D := D).
       - now apply sane_issubst.
       - now apply (ptt_CtxExtendInversion D A),
             (ptt_sane_istype _ B), sane_istype.
@@ -583,7 +584,7 @@ Proof.
     }
 
     (* EqTySubstId *)
-    { capply (@EqTySubstId _ _ _ G D).
+    { config apply @EqTySubstId with (D := D).
       - now apply sane_issubst.
       - now apply (@ptt_sane_isterm D u A), sane_isterm.
       - now apply sane_isterm.
@@ -593,28 +594,28 @@ Proof.
     }
 
     (* EqTySubstEmpty *)
-    { capply (@EqTySubstEmpty _ _ _ G D).
+    { config apply @EqTySubstEmpty with (D := D).
       - now apply sane_issubst.
       - now apply (@ptt_sane_issubst sbs G D), sane_issubst.
       - now apply (@ptt_sane_issubst sbs G D), sane_issubst.
     }
 
     (* EqTySubstUnit *)
-    { capply (@EqTySubstUnit _ _ _ G D).
+    { config apply @EqTySubstUnit with (D := D).
       - now apply sane_issubst.
       - now apply (@ptt_sane_issubst sbs G D), sane_issubst.
       - now apply (@ptt_sane_issubst sbs G D), sane_issubst.
     }
 
     (* EqTySubstBool *)
-    { capply (@EqTySubstBool _ _ _ G D).
+    { config apply @EqTySubstBool with (D := D).
       - now apply sane_issubst.
       - now apply (@ptt_sane_issubst sbs G D), sane_issubst.
       - now apply (@ptt_sane_issubst sbs G D), sane_issubst.
     }
 
     (* EqTyExfalso *)
-    { capply (@EqTyExfalso _ _ _ G A B u).
+    { config apply @EqTyExfalso with (u := u).
       - now apply (@ptt_sane_istype G A), sane_istype.
       - now apply sane_istype.
       - now apply sane_istype.
@@ -647,7 +648,7 @@ Proof.
     }
 
     (* CongTySubst *)
-    { capply (@CongTySubst _ _ _ G D).
+    { config apply @CongTySubst with (D := D).
       - now apply sane_eqsubst.
       - now apply sane_eqtype.
       - now apply (@ptt_sane_eqsubst sbs sbt G D), sane_eqsubst.
@@ -694,7 +695,7 @@ Proof.
     }
 
     (* EqCtxConv *)
-    - { capply (@EqCtxConv _ _ _ G D).
+    - { config apply @EqCtxConv with (G := G).
         - now apply (@ptt_sane_eqctx G D), sane_eqctx.
         - now apply (@ptt_sane_eqctx G D), sane_eqctx.
         - now apply (@ptt_sane_eqterm G u v A), sane_eqterm.
@@ -721,7 +722,7 @@ Proof.
       }
 
     (* EqTrans *)
-    - { capply (@EqTrans _ _ _ G A u v w).
+    - { config apply @EqTrans with (v := v).
         - now apply sane_eqterm.
         - now apply sane_eqterm.
         - now apply (@ptt_sane_eqterm G u v A), sane_eqterm.
@@ -739,7 +740,7 @@ Proof.
       }
 
     (* EqSubstComp *)
-    - { capply (@EqSubstComp _ _ _ G D E A u sbs sbt).
+    - { config apply @EqSubstComp with (D := D) (E := E).
         - now apply sane_isterm.
         - now apply sane_issubst.
         - now apply sane_issubst.
@@ -774,7 +775,7 @@ Proof.
       }
 
     (* EqSubstShiftZero *)
-    - { capply (@EqSubstShiftZero _ _ _ G D).
+    - { config apply @EqSubstShiftZero with (D := D).
         - now apply (@ptt_sane_issubst sbs G D), sane_issubst.
         - now apply (@ptt_sane_issubst sbs G D), sane_issubst.
         - now apply sane_issubst.
@@ -782,7 +783,7 @@ Proof.
       }
 
     (* EqSubstShiftSucc *)
-    - { capply (@EqSubstShiftSucc _ _ _ G D).
+    - { config apply @EqSubstShiftSucc with (D := D).
         - now apply (@ptt_sane_issubst sbs G D), sane_issubst.
         - now apply (@ptt_sane_issubst sbs G D), sane_issubst.
         - now apply (@ptt_sane_isterm D (var k) B), sane_isterm.
@@ -792,7 +793,7 @@ Proof.
       }
 
     (* EqSubstAbs *)
-    - { capply (@EqSubstAbs _ _ _ G D).
+    - { config apply @EqSubstAbs with (D := D).
         - now apply (@ptt_sane_issubst sbs G D), sane_issubst.
         - now apply (@ptt_sane_issubst sbs G D), sane_issubst.
         - now apply (ptt_CtxExtendInversion D A),
@@ -804,7 +805,7 @@ Proof.
       }
 
     (* EqSubstApp *)
-    - { capply (@EqSubstApp _ _ _ G D).
+    - { config apply @EqSubstApp with (D := D).
         - now apply (@ptt_sane_issubst sbs G D), sane_issubst.
         - now apply (@ptt_sane_issubst sbs G D), sane_issubst.
         - now apply (@ptt_sane_isterm D v A), sane_isterm.
@@ -817,7 +818,7 @@ Proof.
       }
 
     (* EqSubstRefl *)
-    - { capply (@EqSubstRefl _ _ _ G D).
+    - { config apply @EqSubstRefl with (D := D).
         - now apply sane_issubst.
         - now apply sane_isterm.
         - now apply (@ptt_sane_issubst sbs G D), sane_issubst.
@@ -826,7 +827,7 @@ Proof.
       }
 
     (* EqSubstJ *)
-    - { capply (@EqSubstJ _ _ _ G D).
+    - { config apply @EqSubstJ with (D := D).
         - now apply (@ptt_sane_issubst sbs G D), sane_issubst.
         - now apply (@ptt_sane_issubst sbs G D), sane_issubst.
         - now apply (@ptt_sane_isterm D v A), sane_isterm.
@@ -839,7 +840,7 @@ Proof.
       }
 
     (* EqSubstExfalso *)
-    - { capply (@EqSubstExfalso _ _ _ G D).
+    - { config apply @EqSubstExfalso with (D := D).
         - now apply (@ptt_sane_issubst sbs G D), sane_issubst.
         - now apply (@ptt_sane_issubst sbs G D), sane_issubst.
         - now apply sane_istype.
@@ -848,28 +849,28 @@ Proof.
       }
 
     (* EqSubstUnit *)
-    - { capply (@EqSubstUnit _ _ _ G D).
+    - { config apply @EqSubstUnit with (D := D).
         - now apply (@ptt_sane_issubst sbs G D), sane_issubst.
         - now apply (@ptt_sane_issubst sbs G D), sane_issubst.
         - now apply sane_issubst.
       }
 
     (* EqSubstTrue *)
-    - { capply (@EqSubstTrue _ _ _ G D).
+    - { config apply @EqSubstTrue with (D := D).
         - now apply sane_issubst.
         - now apply (@ptt_sane_issubst sbs G D), sane_issubst.
         - now apply (@ptt_sane_issubst sbs G D), sane_issubst.
       }
 
     (* EqSubstFalse *)
-    - { capply (@EqSubstFalse _ _ _ G D).
+    - { config apply @EqSubstFalse with (D := D).
         - now apply sane_issubst.
         - now apply (@ptt_sane_issubst sbs G D), sane_issubst.
         - now apply (@ptt_sane_issubst sbs G D), sane_issubst.
       }
 
     (* EqSubstCond *)
-    - { capply (@EqSubstCond _ _ _ G D).
+    - { config apply @EqSubstCond with (D := D).
         - now apply (@ptt_sane_issubst sbs G D), sane_issubst.
         - now apply (@ptt_sane_issubst sbs G D), sane_issubst.
         - now apply sane_issubst.
@@ -880,7 +881,7 @@ Proof.
       }
 
     (* EqTermExfalso *)
-    - { capply (@EqTermExfalso _ _ _ G A u v w).
+    - { config apply @EqTermExfalso with (w := w).
         - now apply (ptt_sane_isterm G u A), sane_isterm.
         - now apply (ptt_sane_isterm G u A), sane_isterm.
         - now apply sane_isterm.
@@ -1042,7 +1043,7 @@ Proof.
       }
 
     (* CongTermSubst *)
-    - { capply (@CongTermSubst _ _ _ G D).
+    - { config apply @CongTermSubst with (D := D).
         - now apply sane_eqsubst.
         - now apply sane_eqterm.
         - now apply (@ptt_sane_eqsubst sbs sbt G D), sane_eqsubst.
