formalization/ett_sanity.v
@@ -16,6 +16,7 @@ Section EttSanity.
 
 Context `{configReflection : config.Reflection}.
 Context `{configSimpleProducts : config.SimpleProducts}.
+Context `{configProdEta : config.ProdEta}.
 
 Theorem sane_issubst sbs G D :
   issubst sbs G D -> isctx G * isctx D.
