formalization/ptt_admissible.v
@@ -11,6 +11,7 @@ Section PttAdmissible.
 Local Instance hasPrecond : config.Precond := {| config.precondFlag := config.Yes |}.
 Context `{configReflection : config.Reflection}.
 Context `{configSimpleProducts : config.SimpleProducts}.
+Context `{configProdEta : config.ProdEta}.
 
 (* Some preliminary lemmata *)
 Lemma EqTyWeakNat :
