formalization/uniqueness.v
@@ -16,6 +16,7 @@ Section Uniqueness.
 
 Context `{configReflection : config.Reflection}.
 Context `{configSimpleProducts : config.SimpleProducts}.
+Context `{configProdEta : config.ProdEta}.
 
 (* Auxiliary inversion lemmas. *)
 
@@ -149,7 +150,7 @@ Ltac doTyConv unique_term' :=
 Ltac doCtxConv D' unique_term' :=
   eapply unique_term' ;
   [ ehyp
-  | capply (@CtxTrans _ _ _ _ D') ; hyp ].
+  | (config apply @CtxTrans with (D := D')) ; hyp ].
 
 Ltac doSubstConv unique_subst' :=
   ceapply CtxTrans ; [
@@ -204,7 +205,7 @@ Proof.
 
     (* H1: TermTyConv *)
     - {
-        capply (@EqTyTrans _ _ _ G _ A B').
+        config apply @EqTyTrans with (B := A).
         + capply EqTySym. hyp.
         + eapply (unique_term_ctx G u A) ; eassumption.
       }
@@ -215,7 +216,7 @@ Proof.
         - eapply unique_term_ctx'.
           + ehyp.
           + ehyp.
-          + capply (@CtxTrans _ _ _ _ D).
+          + config apply @CtxTrans with (D := D).
             * hyp.
             * capply CtxSym. hyp.
         - hyp.
